Common/Char.lean
@@ -1,4 +1,4 @@
 namespace Char
 
-def asDigit (d : Char) (ok : Char.isDigit d = true) : Nat :=
+def asDigit (d : Char) (_ : Char.isDigit d = true) : Nat :=
   d.toNat - 48
